Stratego/JavaExport.thy
@@ -17,10 +17,14 @@ datatype 'a BaseExpressions =
   IntegerConstant int |
   TrueValue |
   FalseValue |
-  MethodCall "'a::JavaExpression" MethodName "'a::JavaExpression list" |
-  Constructor ClassName "'a::JavaExpression list" |
-  InstanceOf "'a BaseExpressions" ClassName VariableName |
-  Equal "'a BaseExpressions" "'a BaseExpressions" |
+  MethodCall "'a::JavaExpression" MethodName "'a::JavaExpression list"
+    ("_._(_)") |
+  Constructor ClassName "'a::JavaExpression list"
+    ("new _(_)") |
+  InstanceOf "'a BaseExpressions" ClassName VariableName
+    ("_ instanceof _ _")|
+  Equal "'a BaseExpressions" "'a BaseExpressions" 
+    (infix "==" 58)|
   ConditionExpression 'a (* |
   Less Expression Expression |
   Negate Expression |
@@ -29,10 +33,16 @@ datatype 'a BaseExpressions =
   Unsupported string*)
 
 datatype ('a) Statement =
-  Assignment VariableName "'a::JavaExpression" |
-  Branch "'a::JavaExpression" "('a) Statement" |
+  Assignment VariableName "'a::JavaExpression" (infix ":=" 56) |
+  Branch "'a::JavaExpression" "('a) Statement" ("if _ {(2//_)//}") |
   Return "'a::JavaExpression" |
   Sequential "('a) Statement list"
+
+syntax
+  "_seq" :: "'a Statement \<Rightarrow> 'a Statement => 'a Statement" (infixr ";//" 55)
+
+translations
+  "_seq x y" == "CONST Sequential [x, y]"
 
 fun intersperse :: "string \<Rightarrow> string list \<Rightarrow> string list" where
   "intersperse i es = foldr (\<lambda>x ys . x # (if ys = [] then ys else i # ys)) es []"
@@ -90,196 +100,45 @@ locale JavaTarget = CompiledRewrites +
   and generate_condition :: "'b \<Rightarrow> 'e::JavaExpression"
   and generate_result :: "'c \<Rightarrow> 'e::JavaExpression"
   and generate_access :: "VarName \<Rightarrow> 'a \<Rightarrow> 'e::JavaExpression list"
-  (*and generate_assignment :: "VarName \<Rightarrow> 'a \<Rightarrow> ('e BaseExpressions) Statement \<Rightarrow> ('e BaseExpressions) Statement"*)
 begin
 
 fun generate_assignment :: 
   "VarName \<Rightarrow> 'a \<Rightarrow> ('e BaseExpressions) Statement \<Rightarrow> ('e BaseExpressions) Statement" where
   "generate_assignment v e s =
     Sequential (
-      [Assignment e' (ConditionExpression ((generate_access (v @ ''c'') e)!i)).
+      [(e' := (ConditionExpression ((generate_access (v @ ''c'') e)!i))).
         (i, e') <- (enumerate 0 (pattern_variables e))] @ [s])"
 
-function (sequential) export_match :: "('a, 'b) MATCH \<Rightarrow> ('e BaseExpressions) Statement 
+fun export_match :: "('a, 'b) MATCH \<Rightarrow> ('e BaseExpressions) Statement 
   \<Rightarrow> ('e BaseExpressions) Statement" where
   "export_match (match v p) r  = 
-    Branch (InstanceOf (Ref v) (class_of_term p) (v @ ''c''))
-      (Sequential [(generate_assignment v p r)])" |
+    if ((Ref v) instanceof (class_of_term p) (v @ ''c'')) {
+      (Sequential [(generate_assignment v p r)])
+    }" |
   "export_match (andthen m1 m2) r = 
     export_match m1 (export_match m2 r)" |
   "export_match (equality v1 v2) r = 
-    Branch (Equal (Ref v1) (Ref v2)) r" |
+    if ((Ref v1) == (Ref v2)) {
+      r
+    }" |
   "export_match (cond sc) r = 
-    Branch (ConditionExpression (generate_condition sc)) r" |
+    if (ConditionExpression (generate_condition sc)) {
+      r
+    }" |
   "export_match noop r = r"
-  apply pat_completeness+
-  by simp+
 
-fun size_conditional :: "(('a, 'b) MATCH \<times> ('e BaseExpressions) Statement) \<Rightarrow> nat" where
-  "size_conditional ((cond c), s) = size_match (cond c) + size_condition c" |
-  "size_conditional (m, s) = size_match m"
+fun generate_rules :: "VarName option \<Rightarrow> ('a, 'b, 'c) Rules \<Rightarrow> ('e BaseExpressions) Statement" where
+  "generate_rules None (base e) = Return (ConditionExpression (generate_result e))" |
+  "generate_rules (Some v) (base e) = (v := (ConditionExpression (generate_result e)))" |
+  "generate_rules v (cond' m r) = export_match m (generate_rules v r)" |
+  "generate_rules v (r1 else r2) = generate_rules v r1; generate_rules v r2" |
+  "generate_rules v (choice rules) = Sequential (map (generate_rules v) rules)" |
+  "generate_rules v (r1 \<then> r2) = 
+    generate_rules (entry_var r2) r1;
+    generate_rules v r2"
 
-termination export_match
-  apply (relation "measures [size_conditional]") apply simp apply simp sorry
+definition "export_rules = generate_rules None"
 
-
-fun export_rules :: "('a, 'b, 'c) Rules \<Rightarrow> ('e BaseExpressions) Statement" where
-  "export_rules (base e) = Return (ConditionExpression (generate_result e))" |
-  "export_rules (cond' m r) = export_match m (export_rules r)" |
-  "export_rules (r1 else r2) = Sequential [export_rules r1, export_rules r2]" |
-  "export_rules (choice rules) = Sequential (map export_rules rules)" |
-  "export_rules (r1 \<then> r2) = Sequential [export_rules r1, export_rules r2]" (* TODO: should modify e *)
 end
-
-
-
-
-fun class_of_term_Arithmetic :: "Arithmetic \<Rightarrow> string" where
-  "class_of_term_Arithmetic (Add x y) = ''AddNode''" |
-  "class_of_term_Arithmetic (Sub x y) = ''SubNode''" |
-  "class_of_term_Arithmetic (UMinus x) = ''UnaryMinusNode''" |
-  "class_of_term_Arithmetic (Number v) = ''ConstantNode''" |
-  "class_of_term_Arithmetic (Variable s) = ''VariableNode''"
-
-datatype JavaCheck =
-  CallMethod1 |
-  CallMethod2 |
-  MethodCall string string |
-  Construct string "JavaCheck list" |
-  VariableExpr string
-
-instantiation "JavaCheck" :: JavaExpression
-begin
-fun expToJava_JavaCheck where
-  "expToJava_JavaCheck CallMethod1 = ''I'm asserting you're a number''" |
-  "expToJava_JavaCheck CallMethod2 = ''I'm asserting you're a subnode''" |
-  "expToJava_JavaCheck (MethodCall ob m) = ob @ ''.'' @ m @ ''()''" |
-  "expToJava_JavaCheck (Construct class args) = ''new '' @ class @ ''('' @ param_list (map expToJava_JavaCheck args) @ '')''" |
-  "expToJava_JavaCheck (VariableExpr v) = v"
-instance ..
-end
-
-fun generate_condition_Arithmetic :: "ArithmeticCondition \<Rightarrow> JavaCheck" where
-  "generate_condition_Arithmetic (IsSub e) = CallMethod2" |
-  "generate_condition_Arithmetic (IsNumber e) = CallMethod1"
-
-fun generate_Arithmetic :: "Arithmetic \<Rightarrow> JavaCheck" where
-  "generate_Arithmetic (Add x y) = Construct ''AddNode'' (map generate_Arithmetic [x, y])" |
-  "generate_Arithmetic (Sub x y) = Construct ''SubNode'' (map generate_Arithmetic [x, y])" |
-  "generate_Arithmetic (UMinus x) = Construct ''UnaryMinusNode'' (map generate_Arithmetic [x])" |
-  "generate_Arithmetic (Number v) = Construct ''ConstantNode'' []" |
-  "generate_Arithmetic (Variable s) = VariableExpr s"
-
-fun generate_result_Arithmetic :: "Transformer \<Rightarrow> JavaCheck" where
-  "generate_result_Arithmetic (UnaryMinus e) = CallMethod1" |
-  "generate_result_Arithmetic (Plus e1 e2) = CallMethod2" |
-  "generate_result_Arithmetic (Result e) = generate_Arithmetic e"
-
-fun generate_access_Arithmetic :: "VarName \<Rightarrow> Arithmetic \<Rightarrow> JavaCheck list" where
-  "generate_access_Arithmetic v (Add x y) = 
-    [(MethodCall v ''getX''),
-     (MethodCall v ''getY'')]" |
-  "generate_access_Arithmetic v (Sub x y) = 
-    [(MethodCall v ''getX''),
-     (MethodCall v ''getY'')]" |
-  "generate_access_Arithmetic v (UMinus x) = [(MethodCall v ''getValue'')]" |
-  "generate_access_Arithmetic v (Number val) = []" |
-  "generate_access_Arithmetic v (Variable s) = []"
-
-(*
-  "export_assignments v (UnaryPattern op v1) s = Sequential
-    [Assignment v1 (MethodCall (Ref (v + STR ''c'')) ''getValue'' []), s]" |
-  "export_assignments v (BinaryPattern op v1 v2) s = Sequential
-    [Assignment v1 (MethodCall (Ref (v + STR ''c'')) ''getX'' []),
-     Assignment v2 (MethodCall (Ref (v + STR ''c'')) ''getY'' []), s]" |
-  "export_assignments v (ConditionalPattern v1 v2 v3) s = Sequential
-    [Assignment v1 (MethodCall (Ref (v + STR ''c'')) ''condition'' []),
-     Assignment v2 (MethodCall (Ref (v + STR ''c'')) ''trueValue'' []),
-     Assignment v3 (MethodCall (Ref (v + STR ''c'')) ''falseValue'' []), s]" |
-  "export_assignments v (ConstantPattern val) s =
-    Branch (InstanceOf (MethodCall (Ref (v + STR ''c'')) ''getValue'' []) ''PrimitiveConstant'' (v + STR ''cd''))
-    (Branch (Equal (MethodCall (Ref (v + STR ''cd'')) ''asLong'' []) (export_value val)) s)" |
-  "export_assignments v (ConstantVarPattern var) s =
-    Branch (Equal (MethodCall (Ref (v + STR ''c'')) ''getValue'' []) (Ref var)) s" |
-  "export_assignments v (VariablePattern var) s =
-    Return (Unsupported ''export_assignments for VariablePattern'')" 
-*)
-
-setup \<open>Locale_Code.open_block\<close>
-interpretation Arithmetic: JavaTarget
-  size_Arithmetic
-  "eval_condition"
-  "ground_condition"
-  "is_ground_condition"
-  "eval_transformer"
-  "ground_transformer"
-  "is_ground_transformer"
-  rewrite_Arithmetic
-  match_Arithmetic
-  varof_Arithmetic
-  var_Arithmetic
-  subexprs_Arithmetic
-  chain_Arithmetic
-  class_of_term_Arithmetic
-  generate_condition_Arithmetic
-  generate_result_Arithmetic
-  generate_access_Arithmetic
-proof
-  fix e :: Arithmetic
-  show "\<forall>e' \<in> set (subexprs_Arithmetic e). size_Arithmetic e > size_Arithmetic e'"
-    by (cases e; simp)
-next
-  fix f :: "Arithmetic \<Rightarrow> Arithmetic"
-  fix e :: Arithmetic
-  show "map f (subexprs_Arithmetic e) = subexprs_Arithmetic (snd (chain_Arithmetic (\<lambda>e a. (plus a 1, f e)) e 0))"
-    by (cases e; simp)
-next
-  fix f :: "Arithmetic \<Rightarrow> Arithmetic"
-  fix e :: Arithmetic
-  show "length (subexprs_Arithmetic e) = fst (chain_Arithmetic (\<lambda>e a. (plus a 1, f e)) e 0)"
-    by (cases e; simp)
-qed
-setup \<open>Locale_Code.close_block\<close>
-
-definition "export_rules = Arithmetic.export_rules"
-
-
-value "export_rules"
-
-definition "join = Arithmetic.join"
-(*definition "compile' = ArithmeticCompiled.compile'"*)
-definition "generate = Arithmetic.generate"
-definition "match_pattern = Arithmetic.match_pattern"
-definition "optimized_export = Arithmetic.optimized_export"
-
-export_code "optimized_export" checking SML
-
-definition Identity where
-  "Identity = generate 
-    (Add
-      (var ''x'')
-      (Number 0))
-    (Result (var ''x''))"
-
-value "Identity"
-text "@{value[display] \<open>Identity\<close>}"
-value "optimized_export Identity"
-text "@{value[display] \<open>optimized_export Identity\<close>}"
-
-text \<open>@{text "const x + const y \<longrightarrow> const (x + y)"}\<close>
-definition Evaluate where
-  "Evaluate = generate 
-    (Add
-      (var ''x'')
-      (var ''y''))
-    (Plus (var ''x'') (var ''y''))"
-(* doesn't support constant evaluation *)
-value "Evaluate"
-value "(optimized_export (Evaluate))"
-
-
-value "export_rules (optimized_export (choice [Identity, Evaluate]))"
-
-value "statementToJava 0 (export_rules (optimized_export (choice [Identity, Evaluate])))"
 
 end
