Stratego/Stratego.thy
@@ -3,9 +3,6 @@ theory Stratego
   imports Main "HOL-Library.Finite_Map" "HOL-Library.Word" Locale_Code.Locale_Code "HOL-Library.Monad_Syntax"
 begin
 
-no_notation plus (infixl "+" 65)
-no_notation less ("(_/ < _)"  [51, 51] 50)
-
 text \<open>
 We generalize the concept of a datatype that can be rewritten using Stratego
 using the @{term Rewritable} class.
@@ -39,7 +36,8 @@ locale Rewritable =
   and ground_result :: "'c \<Rightarrow> (string \<rightharpoonup> 'a) \<Rightarrow> 'c"
   and is_ground_result :: "'c \<Rightarrow> bool"
  +
-  
+  fixes subexprs :: "'a \<Rightarrow> 'a list"
+  fixes chain :: "('a \<Rightarrow> nat \<Rightarrow> (nat \<times> 'a)) \<Rightarrow> 'a \<Rightarrow> nat \<Rightarrow> (nat \<times> 'a)"
   fixes rewrite :: "('a \<Rightarrow> 'a) \<Rightarrow> 'a \<Rightarrow> 'a"
   fixes match_term :: "'a \<Rightarrow> 'a \<Rightarrow> ((string, 'a) fmap) option"
   fixes varof :: "'a \<Rightarrow> string option"
@@ -50,8 +48,18 @@ locale Rewritable =
 
   fixes transform :: "'c \<Rightarrow> 'a \<Rightarrow> 'a option"*)
 
-  assumes "a' \<subseteq>\<^sub>m a \<Longrightarrow> is_ground_condition (ground_condition e a') \<Longrightarrow> ground_condition e a' = ground_condition e a"
+  assumes "a' \<subseteq>\<^sub>m a \<Longrightarrow> is_ground_condition (ground_condition c a') \<Longrightarrow> ground_condition c a' = ground_condition c a"
+  assumes shrinks: "\<forall>e' \<in> set (subexprs e). size e > size e'"
+  assumes "map f (subexprs e) = subexprs (snd (chain (\<lambda>e a. (plus a 1, f e)) e 0))"
+  assumes "length (subexprs e) = fst (chain (\<lambda>e a. (plus a 1, f e)) e 0)"
+  assumes "eval_condition c = None \<equiv> \<not>(is_ground_condition c)"
 begin
+(*fun rewrite :: "('a \<Rightarrow> 'a) \<Rightarrow> 'a \<Rightarrow> 'a" where
+  "rewrite f xs = snd (chain (\<lambda>e a. (plus a 1, f e)) xs (0::nat))"*)
+
+no_notation plus (infixl "+" 65)
+no_notation less ("(_/ < _)"  [51, 51] 50)
+
 subsection "Rewrite Language"
 datatype ('e, 'cond, 't) Strategy =
   id | \<comment> \<open>identity operator\<close>
@@ -138,288 +146,5 @@ fun chain_list :: "'b \<Rightarrow> ('a \<Rightarrow> 'b \<Rightarrow> ('b \<tim
   "chain_list a f (x # xs) =
     (let (a', x') = f x a in
     (let (a'', xs') = (chain_list a' f xs) in (a'', x' # xs')))"
-
-subsection "Example: Simple Arithmetic Rewrites"
-
-datatype (discs_sels) Arithmetic =
-  Add Arithmetic Arithmetic |
-  Sub Arithmetic Arithmetic |
-  UMinus Arithmetic |
-  Number int |
-  Variable string
-
-
-fun compatible :: "('a, 'b) fmap \<Rightarrow> ('a, 'b) fmap \<Rightarrow> bool" where
-  "compatible s1 s2 = (\<forall>x \<in> fset (fmdom s1) . fmlookup s2 x \<noteq> None \<longrightarrow> fmlookup s1 x = fmlookup s2 x)"
-
-(*fun union :: "(('a, 'b) fmap) option \<Rightarrow> (('a, 'b) fmap) option \<Rightarrow> (('a, 'b) fmap) option" where
-  "union s1 s2 = 
-      (case s1 of
-       None \<Rightarrow> None |
-       Some s1' \<Rightarrow>
-           (case s2 of
-            None \<Rightarrow> None |
-            Some s2' \<Rightarrow> (if compatible s1' s2' then Some (s1' ++\<^sub>f s2') else None)
-           )
-      )"*)
-
-fun union :: "(('a, 'b) fmap) option \<Rightarrow> (('a, 'b) fmap) option \<Rightarrow> (('a, 'b) fmap) option" where
-  "union s1 s2 = do {
-    s1' <- s1;
-    s2' <- s2;
-    if compatible s1' s2' then Some (s1' ++\<^sub>f s2') else None
-  }"
-
-fun rewrite_Arithmetic :: "(Arithmetic \<Rightarrow> Arithmetic) \<Rightarrow> Arithmetic \<Rightarrow> Arithmetic" where
-  "rewrite_Arithmetic f (Add x y) = f (Add (rewrite_Arithmetic f x) (rewrite_Arithmetic f y))" |
-  "rewrite_Arithmetic f (Sub x y) = f (Sub (rewrite_Arithmetic f x) (rewrite_Arithmetic f y))" |
-  "rewrite_Arithmetic f (UMinus x) = f (UMinus (rewrite_Arithmetic f x))" |
-  "rewrite_Arithmetic f (Number v) = f (Number v)" |
-  "rewrite_Arithmetic f (Variable s) = f (Variable s)"
-
-fun match_Arithmetic :: "Arithmetic \<Rightarrow> Arithmetic \<Rightarrow> ((string, Arithmetic) fmap) option" where
-  "match_Arithmetic (Add x y) (Add x' y') = 
-    union (match_Arithmetic x x') (match_Arithmetic y y')" |
-  "match_Arithmetic (Sub x y) (Sub x' y') =
-    union (match_Arithmetic x x') (match_Arithmetic y y')" |
-  "match_Arithmetic (UMinus x) (UMinus x') =
-    (match_Arithmetic x x')" |
-  "match_Arithmetic (Number v) (Number v') = (if v = v' then Some (fmempty) else None)" |
-  "match_Arithmetic (Variable v) e = Some (fmupd v e fmempty)" |
-  "match_Arithmetic _ _ = None"
-
-fun varof_Arithmetic :: "Arithmetic \<Rightarrow> string option" where
-  "varof_Arithmetic (Variable s) = Some s" |
-  "varof_Arithmetic _ = None"
-
-fun var_Arithmetic :: "string \<Rightarrow> Arithmetic" where
-  "var_Arithmetic v = Variable v"
-
-fun subexprs_Arithmetic :: "Arithmetic \<Rightarrow> Arithmetic list" where
-  "subexprs_Arithmetic (Add x y) = [x, y]" |
-  "subexprs_Arithmetic (Sub x y) = [x, y]" |
-  "subexprs_Arithmetic (UMinus x) = [x]" |
-  "subexprs_Arithmetic (Number v) = []" |
-  "subexprs_Arithmetic (Variable s) = []"
-
-fun chain_Arithmetic :: "(Arithmetic \<Rightarrow> nat \<Rightarrow> (nat \<times> Arithmetic)) \<Rightarrow> Arithmetic \<Rightarrow> nat \<Rightarrow> (nat \<times> Arithmetic)" where
-  "chain_Arithmetic f (Add x y) n =
-    (let (n', x') = f x n in
-    (let (n'', y') = f y n' in
-      (n'', Add x' y')))" |
-  "chain_Arithmetic f (Sub x y) n =
-    (let (n', x') = f x n in
-    (let (n'', y') = f y n' in
-      (n'', Sub x' y')))" |
-  "chain_Arithmetic f (UMinus x) n =
-    (let (n', x') = f x n in
-      (n', UMinus x'))" |
-  "chain_Arithmetic f (Number v) n = (n, (Number v))" |
-  "chain_Arithmetic f (Variable s) n = (n, (Variable s))"
-
-(*
-locale ConditionalRewritable = Rewritable +
-  fixes condition :: "'b \<Rightarrow> 'a Strategy"
-  fixes eval_condition :: "'b \<Rightarrow> bool"
-  fixes ground :: "'b \<Rightarrow> 'a Binding \<Rightarrow> 'b option"
-begin
-
-lemma eval_condition[code]:
-  "eval (condition e) (s, state) = (case (ground e state) of 
-                                    Some e' \<Rightarrow> ((s, state), eval_condition e') |
-                                    None \<Rightarrow> ((s, state), False))"
-  sorry
-
-end
-*)
-
-datatype ArithmeticCondition =
-  IsSub Arithmetic |
-  IsNumber Arithmetic
-
-fun eval_condition :: "ArithmeticCondition \<Rightarrow> bool option" where
-  "eval_condition (IsSub (Sub x y)) = Some True" |
-  "eval_condition (IsNumber (Number v)) = Some True" |
-  "eval_condition _ = Some False"
-
-fun ground_condition :: "ArithmeticCondition \<Rightarrow> (string \<rightharpoonup> Arithmetic) \<Rightarrow> ArithmeticCondition" where
-  "ground_condition (IsSub (Variable v)) f = (case f v of 
-                                              Some v' \<Rightarrow> (IsSub v') |
-                                              None \<Rightarrow> (IsSub (Variable v)))" |
-  "ground_condition (IsNumber (Variable v)) f = (case f v of 
-                                              Some v' \<Rightarrow> (IsNumber v') |
-                                              None \<Rightarrow> (IsNumber (Variable v)))" |
-  "ground_condition e f = e"
-
-fun is_ground_condition :: "ArithmeticCondition \<Rightarrow> bool" where
-  "is_ground_condition (IsSub e) = is_Variable e" |
-  "is_ground_condition (IsNumber e) = is_Variable e"
-
-datatype Transformer =
-  UnaryMinus Arithmetic |
-  Plus Arithmetic Arithmetic |
-  Result Arithmetic
-
-fun eval_transformer :: "Transformer \<Rightarrow> Arithmetic option" where
-  "eval_transformer (UnaryMinus (Number x)) = Some (Number (-x))" |
-  "eval_transformer (Plus (Number x) (Number y)) = Some (Number (plus x y))" |
-  "eval_transformer (Result a) = Some a" |
-  "eval_transformer _ = None"
-
-fun ground_transformer :: "Transformer \<Rightarrow> (string \<rightharpoonup> Arithmetic) \<Rightarrow> Transformer" where
-  "ground_transformer (UnaryMinus (Variable v)) f = (case f v of 
-                                              Some v' \<Rightarrow> (UnaryMinus v') |
-                                              None \<Rightarrow> (UnaryMinus (Variable v)))" |
-  "ground_transformer (Plus (Variable x) (Variable y)) f = (case f x of 
-                                              Some x' \<Rightarrow> (
-                                                case f y of Some y' \<Rightarrow> (Plus x' y')
-                                                            | None \<Rightarrow> (Plus (Variable x) (Variable y)))
-                                              | None \<Rightarrow> (Plus (Variable x) (Variable y)))" |
-  "ground_transformer (Result (Variable v)) f = (case f v of 
-                                              Some v' \<Rightarrow> (Result v') |
-                                              None \<Rightarrow> (Result (Variable v)))" |
-  "ground_transformer e f = e"
-
-fun is_ground_transformer :: "Transformer \<Rightarrow> bool" where
-  "is_ground_transformer (UnaryMinus e) = is_Variable e" |
-  "is_ground_transformer (Plus e1 e2) = (is_Variable e1 \<or> is_Variable e2)" |
-  "is_ground_transformer (Result e) = is_Variable e"
-
-print_locale Rewritable
-setup \<open>Locale_Code.open_block\<close>
-interpretation Arithmetic: Rewritable
-  size_Arithmetic
-  "eval_condition"
-  "ground_condition"
-  "is_ground_condition"
-  "eval_transformer"
-  "ground_transformer"
-  "is_ground_transformer"
-  rewrite_Arithmetic
-  match_Arithmetic
-  varof_Arithmetic
-  var_Arithmetic
-  apply standard sorry
-(*
-  by (smt (z3) domIff ground_condition.elims ground_condition.simps(1) ground_condition.simps(2) map_le_def option.case_eq_if option.distinct(1))
-*)
-
-setup \<open>Locale_Code.close_block\<close>
-
-
-(*
-setup \<open>Locale_Code.open_block\<close>
-interpretation ArithmeticCondition : ConditionalRewritable
-  size_Arithmetic
-  rewrite_Arithmetic
-  match_Arithmetic
-  varof_Arithmetic
-  var_Arithmetic
-  subexprs_Arithmetic
-  chain_Arithmetic
-  condition
-  
-  by standard
-setup \<open>Locale_Code.close_block\<close>
-*)
-
-
-subsubsection "Rewrite Rules"
-
-definition "eval = Arithmetic.eval"
-definition "var = var_Arithmetic"
-
-notation Arithmetic.conditional_rewrite_to ("_ \<rightarrow> _ where _")
-notation Arithmetic.not ("not _")
-notation Arithmetic.condition ("condition _")
-notation Arithmetic.func ("func _")
-
-type_synonym StrategyRule = "(Arithmetic, ArithmeticCondition, Transformer) Arithmetic.Strategy"
-
-
-export_code "eval" checking SML
-
-definition RedundantAdd :: "StrategyRule" where
-  "RedundantAdd = ((Add (var ''b'') (Number 0)) \<rightarrow> (var ''b''))"
-
-value "eval (RedundantAdd) ((Add (Number 10) (Number 10)), fmempty)"
-
-definition RedundantSub :: "StrategyRule" where
-  "RedundantSub = ((Sub (var ''a'') (Number 0)) \<rightarrow> (var ''a'') where condition (IsSub (var ''a'')))"
-
-value "eval (RedundantSub) ((Sub (Number 10) (Number 0)), fmempty)"
-value "eval (RedundantSub) ((Sub (Sub (Number 100) (Number 1000)) (Number 0)), fmempty)"
-
-
-definition ShiftConstRight :: "StrategyRule" where
-  "ShiftConstRight = 
-    ((Add (var ''a'') (var ''b'')) \<rightarrow> (Add (var ''b'') (var ''a''))
-      where ((var ''a'')!; not (Number 0?)))"
-
-definition ShiftConstRight2 :: "StrategyRule" where
-  "ShiftConstRight2 = 
-    ((Add (var ''a'') (var ''b'')) \<rightarrow> (Add (var ''b'') (var ''a''))
-      where (condition (IsNumber (var ''a''))))"
-
-definition EvalMinus :: "StrategyRule" where
-  "EvalMinus = 
-    ((UMinus (Variable ''a'')) \<rightarrow> ((Variable ''b''))
-      where (condition (IsNumber (Variable ''a'')); func (UnaryMinus (Variable ''a'')); (Variable ''b'')?))"
-
-definition EvalMinus1 :: "StrategyRule" where
-  "EvalMinus1 =
-    (UMinus (Variable ''a'')) \<rightarrow> Variable ''b''
-      where (condition (IsNumber (Variable ''a'')); (Variable ''b'') := (func (UnaryMinus (Variable ''a''))))"
-
-definition EvalAdd :: "StrategyRule" where
-  "EvalAdd =
-    ((Add (Variable ''a'') (Variable ''b'')) \<rightarrow> ((Variable ''c''))
-      where (
-        (condition (IsNumber (Variable ''a'')));
-        (condition (IsNumber (Variable ''a'')));
-        ((Variable ''c'') := (func (Plus (Variable ''a'') (Variable ''b''))))
-      ))"
-
-subsubsection "Rewrite Application"
-
-text "
-The combination of @{term RedundantAdd} and @{term RedundantSub}
-provides us a rule that will eliminate zero in either add or sub expressions.
-It is defined as @{term \<open>RedundantAdd <+ RedundantSub\<close>}.
-The expanded version of this rule is:
-
-@{value \<open>RedundantAdd <+ RedundantSub\<close>}"
-
-\<comment> \<open>Failing to apply the rule\<close>
-value "eval (RedundantAdd <+ RedundantSub) ((Add (Number 10) (Number 10)), fmempty)"
-text \<open>@{value "eval (RedundantAdd <+ RedundantSub) ((Add (Number 10) (Number 10)), fmempty)"}\<close>
-
-\<comment> \<open>Successful application\<close>
-value "eval (RedundantAdd <+ RedundantSub) ((Add (Number 10) (Number 0)), fmempty)"
-text \<open>@{value "eval (RedundantAdd <+ RedundantSub) ((Add (Number 10) (Number 0)), fmempty)"}\<close>
-
-\<comment> \<open>Successful application in the second rule\<close>
-value "eval (RedundantSub <+ RedundantAdd) ((Add (Number 10) (Number 0)), fmempty)"
-text \<open>@{value "eval (RedundantSub <+ RedundantAdd) ((Add (Number 10) (Number 0)), fmempty)"}\<close>
-
-value "ShiftConstRight"
-value "eval ShiftConstRight ((Add (Number 0) (Number 10)), fmempty)"
-value "eval ShiftConstRight ((Add (Number 10) (Add (Number 10) (Number 20))), fmempty)"
-value "eval ShiftConstRight ((Add (Number 10) (Number 120)), fmempty)"
-
-value "eval ShiftConstRight2 ((Add (Number 0) (Number 10)), fmempty)"
-value "eval ShiftConstRight2 ((Add (Number 10) (Add (Number 10) (Number 20))), fmempty)"
-value "eval ShiftConstRight2 ((Add (Number 10) (Number 120)), fmempty)"
-
-value "eval EvalMinus ((UMinus (Number 10)), fmempty)"
-value "eval EvalMinus ((UMinus (Add (Number 10) (Number 10))), fmempty)"
-text \<open>@{value "eval EvalMinus ((UMinus (Number 10)), fmempty)"}\<close>
-
-value "eval EvalAdd ((UMinus (Number 10)), fmempty)"
-value "eval EvalAdd ((Add (Number 10) (Number 10)), fmempty)"
-text \<open>@{value "eval EvalAdd ((Add (Number 10) (Number 10)), fmempty)"}\<close>
-
-notation plus (infixl "+" 65)
-notation less ("(_/ < _)"  [51, 51] 50)
 
 end
