Stratego/ArithmeticExample.thy
@@ -1,0 +1,473 @@
+theory ArithmeticExample
+  imports JavaExport
+begin
+
+
+subsection "Example: Simple Arithmetic Rewrites"
+
+datatype (discs_sels) Arithmetic =
+  Add Arithmetic Arithmetic |
+  Sub Arithmetic Arithmetic |
+  UMinus Arithmetic |
+  Number int |
+  Variable string
+
+fun compatible :: "('a, 'b) fmap \<Rightarrow> ('a, 'b) fmap \<Rightarrow> bool" where
+  "compatible s1 s2 = (\<forall>x \<in> fset (fmdom s1) . fmlookup s2 x \<noteq> None \<longrightarrow> fmlookup s1 x = fmlookup s2 x)"
+
+fun union :: "(('a, 'b) fmap) option \<Rightarrow> (('a, 'b) fmap) option \<Rightarrow> (('a, 'b) fmap) option" where
+  "union s1 s2 = do {
+    s1' <- s1;
+    s2' <- s2;
+    if compatible s1' s2' then Some (s1' ++\<^sub>f s2') else None
+  }"
+
+fun match_Arithmetic :: "Arithmetic \<Rightarrow> Arithmetic \<Rightarrow> ((string, Arithmetic) fmap) option" where
+  "match_Arithmetic (Add x y) (Add x' y') = 
+    union (match_Arithmetic x x') (match_Arithmetic y y')" |
+  "match_Arithmetic (Sub x y) (Sub x' y') =
+    union (match_Arithmetic x x') (match_Arithmetic y y')" |
+  "match_Arithmetic (UMinus x) (UMinus x') =
+    (match_Arithmetic x x')" |
+  "match_Arithmetic (Number v) (Number v') = (if v = v' then Some (fmempty) else None)" |
+  "match_Arithmetic (Variable v) e = Some (fmupd v e fmempty)" |
+  "match_Arithmetic _ _ = None"
+
+fun varof_Arithmetic :: "Arithmetic \<Rightarrow> string option" where
+  "varof_Arithmetic (Variable s) = Some s" |
+  "varof_Arithmetic _ = None"
+
+fun var_Arithmetic :: "string \<Rightarrow> Arithmetic" where
+  "var_Arithmetic v = Variable v"
+
+fun rewrite_Arithmetic :: "(Arithmetic \<Rightarrow> Arithmetic) \<Rightarrow> Arithmetic \<Rightarrow> Arithmetic" where
+  "rewrite_Arithmetic f (Add x y) = f (Add (rewrite_Arithmetic f x) (rewrite_Arithmetic f y))" |
+  "rewrite_Arithmetic f (Sub x y) = f (Sub (rewrite_Arithmetic f x) (rewrite_Arithmetic f y))" |
+  "rewrite_Arithmetic f (UMinus x) = f (UMinus (rewrite_Arithmetic f x))" |
+  "rewrite_Arithmetic f (Number v) = f (Number v)" |
+  "rewrite_Arithmetic f (Variable s) = f (Variable s)"
+
+fun subexprs_Arithmetic :: "Arithmetic \<Rightarrow> Arithmetic list" where
+  "subexprs_Arithmetic (Add x y) = [x, y]" |
+  "subexprs_Arithmetic (Sub x y) = [x, y]" |
+  "subexprs_Arithmetic (UMinus x) = [x]" |
+  "subexprs_Arithmetic (Number v) = []" |
+  "subexprs_Arithmetic (Variable s) = []"
+
+fun chain_Arithmetic :: "(Arithmetic \<Rightarrow> nat \<Rightarrow> (nat \<times> Arithmetic)) \<Rightarrow> Arithmetic \<Rightarrow> nat \<Rightarrow> (nat \<times> Arithmetic)" where
+  "chain_Arithmetic f (Add x y) n =
+    (let (n', x') = f x n in
+    (let (n'', y') = f y n' in
+      (n'', Add x' y')))" |
+  "chain_Arithmetic f (Sub x y) n =
+    (let (n', x') = f x n in
+    (let (n'', y') = f y n' in
+      (n'', Sub x' y')))" |
+  "chain_Arithmetic f (UMinus x) n =
+    (let (n', x') = f x n in
+      (n', UMinus x'))" |
+  "chain_Arithmetic f (Number v) n = (n, (Number v))" |
+  "chain_Arithmetic f (Variable s) n = (n, (Variable s))"
+
+datatype ArithmeticCondition =
+  IsSub Arithmetic |
+  IsNumber Arithmetic
+
+fun eval_condition :: "ArithmeticCondition \<Rightarrow> bool option" where
+  "eval_condition (IsSub (Sub x y)) = Some True" |
+  "eval_condition (IsNumber (Number v)) = Some True" |
+  "eval_condition (IsSub (Variable v)) = None" |
+  "eval_condition (IsNumber (Variable v)) = None" |
+  "eval_condition _ = Some False"
+
+fun ground_condition :: "ArithmeticCondition \<Rightarrow> (string \<rightharpoonup> Arithmetic) \<Rightarrow> ArithmeticCondition" where
+  "ground_condition (IsSub (Variable v)) f = (case f v of 
+                                              Some v' \<Rightarrow> (IsSub v') |
+                                              None \<Rightarrow> (IsSub (Variable v)))" |
+  "ground_condition (IsNumber (Variable v)) f = (case f v of 
+                                              Some v' \<Rightarrow> (IsNumber v') |
+                                              None \<Rightarrow> (IsNumber (Variable v)))" |
+  "ground_condition e f = e"
+
+fun is_ground_condition :: "ArithmeticCondition \<Rightarrow> bool" where
+  "is_ground_condition (IsSub e) = (\<not>(is_Variable e))" |
+  "is_ground_condition (IsNumber e) = (\<not>(is_Variable e))"
+
+datatype Transformer =
+  UnaryMinus Arithmetic |
+  Plus Arithmetic Arithmetic |
+  Result Arithmetic
+
+fun eval_transformer :: "Transformer \<Rightarrow> Arithmetic option" where
+  "eval_transformer (UnaryMinus (Number x)) = Some (Number (-x))" |
+  "eval_transformer (Plus (Number x) (Number y)) = Some (Number (plus x y))" |
+  "eval_transformer (Result a) = Some a" |
+  "eval_transformer _ = None"
+
+fun ground_transformer :: "Transformer \<Rightarrow> (string \<rightharpoonup> Arithmetic) \<Rightarrow> Transformer" where
+  "ground_transformer (UnaryMinus (Variable v)) f = (case f v of 
+                                              Some v' \<Rightarrow> (UnaryMinus v') |
+                                              None \<Rightarrow> (UnaryMinus (Variable v)))" |
+  "ground_transformer (Plus (Variable x) (Variable y)) f = (case f x of 
+                                              Some x' \<Rightarrow> (
+                                                case f y of Some y' \<Rightarrow> (Plus x' y')
+                                                            | None \<Rightarrow> (Plus (Variable x) (Variable y)))
+                                              | None \<Rightarrow> (Plus (Variable x) (Variable y)))" |
+  "ground_transformer (Result (Variable v)) f = (case f v of 
+                                              Some v' \<Rightarrow> (Result v') |
+                                              None \<Rightarrow> (Result (Variable v)))" |
+  "ground_transformer e f = e"
+
+fun is_ground_transformer :: "Transformer \<Rightarrow> bool" where
+  "is_ground_transformer (UnaryMinus e) = is_Variable e" |
+  "is_ground_transformer (Plus e1 e2) = (is_Variable e1 \<or> is_Variable e2)" |
+  "is_ground_transformer (Result e) = is_Variable e"
+
+setup \<open>Locale_Code.open_block\<close>
+interpretation Arithmetic: CompiledRewrites
+  size_Arithmetic
+  "eval_condition"
+  "ground_condition"
+  "is_ground_condition"
+  "eval_transformer"
+  "ground_transformer"
+  "is_ground_transformer"
+  subexprs_Arithmetic
+  chain_Arithmetic
+  rewrite_Arithmetic
+  match_Arithmetic
+  varof_Arithmetic
+  var_Arithmetic
+proof
+  fix c :: ArithmeticCondition
+  fix a' a :: "(string \<rightharpoonup> Arithmetic)"
+  assume sub: "a' \<subseteq>\<^sub>m a"
+  assume ground: "is_ground_condition (ground_condition c a')"
+  show "ground_condition c a' = ground_condition c a"
+    using sub ground 
+    apply (induction c a rule: ground_condition.induct)
+    defer defer apply simp+
+    subgoal premises prem for e f
+    proof (cases "a' e")
+      case None
+      then have "\<not>(is_ground_condition (case a' e of None \<Rightarrow> IsSub (Variable e) | Some x \<Rightarrow> IsSub x))"
+        by simp
+      then show ?thesis using prem by blast
+    next
+      case (Some a)
+      then have "a' e = f e" using prem(1)
+        by (metis domIff map_le_def option.distinct(1))
+      then show ?thesis by simp
+    qed
+    apply simp
+    subgoal premises prem for e f
+    proof (cases "a' e")
+      case None
+      then have "\<not>(is_ground_condition (case a' e of None \<Rightarrow> IsNumber (Variable e) | Some x \<Rightarrow> IsNumber x))"
+        by simp
+      then show ?thesis using prem by blast
+    next
+      case (Some a)
+      then have "a' e = f e" using prem(1)
+        by (metis domIff map_le_def option.distinct(1))
+      then show ?thesis by simp
+    qed
+    done
+next
+  fix e :: Arithmetic
+  show "\<forall>e' \<in> set (subexprs_Arithmetic e). size_Arithmetic e > size_Arithmetic e'"
+    by (cases e; simp)
+next
+  fix f :: "Arithmetic \<Rightarrow> Arithmetic"
+  fix e :: Arithmetic
+  show "map f (subexprs_Arithmetic e) = subexprs_Arithmetic (snd (chain_Arithmetic (\<lambda>e a. (plus a 1, f e)) e 0))"
+    by (cases e; simp)
+next
+  fix f :: "Arithmetic \<Rightarrow> Arithmetic"
+  fix e :: Arithmetic
+  show "length (subexprs_Arithmetic e) = fst (chain_Arithmetic (\<lambda>e a. (plus a 1, f e)) e 0)"
+    by (cases e; simp)
+next
+  fix c :: "ArithmeticCondition"
+  have lhs: "eval_condition c = None \<Longrightarrow> (\<not> is_ground_condition c)"
+  subgoal premises e
+  proof (cases c)
+    case (IsSub x1)
+    then show ?thesis using e by (cases x1; auto) 
+  next
+    case (IsNumber x2)
+    then show ?thesis using e by (cases x2; auto)
+  qed
+  done
+  have rhs: "(\<not> is_ground_condition c) \<Longrightarrow> eval_condition c = None"
+  subgoal premises e
+  proof (cases c)
+    case (IsSub x1)
+    then show ?thesis using e by (cases x1; auto) 
+  next
+    case (IsNumber x2)
+    then show ?thesis using e by (cases x2; auto)
+  qed
+  done
+  from lhs rhs show "eval_condition c = None \<equiv> (\<not> is_ground_condition c)"
+    by linarith
+qed
+setup \<open>Locale_Code.close_block\<close>
+
+
+subsubsection "Stratego Rules"
+
+definition "eval = Arithmetic.eval"
+definition "var = var_Arithmetic"
+
+notation Arithmetic.conditional_rewrite_to ("_ \<rightarrow> _ where _")
+notation Arithmetic.not ("not _")
+notation Arithmetic.condition ("condition _")
+notation Arithmetic.func ("func _")
+
+type_synonym StrategyRule = "(Arithmetic, ArithmeticCondition, Transformer) Arithmetic.Strategy"
+
+code_datatype fmap_of_list
+lemma fmlookup_of_list[code]: "fmlookup (fmap_of_list m) = map_of m"
+  by (simp add: fmlookup_of_list)
+
+export_code "eval" checking SML
+
+definition RedundantAdd :: "StrategyRule" where
+  "RedundantAdd = ((Add (var ''b'') (Number 0)) \<rightarrow> (var ''b''))"
+
+value "eval (RedundantAdd) ((Add (Number 10) (Number 10)), fmempty)"
+
+definition RedundantSub :: "StrategyRule" where
+  "RedundantSub = ((Sub (var ''a'') (Number 0)) \<rightarrow> (var ''a'') where condition (IsSub (var ''a'')))"
+
+value "eval (RedundantSub) ((Sub (Number 10) (Number 0)), fmempty)"
+value "eval (RedundantSub) ((Sub (Sub (Number 100) (Number 1000)) (Number 0)), fmempty)"
+
+
+definition ShiftConstRight :: "StrategyRule" where
+  "ShiftConstRight = 
+    ((Add (var ''a'') (var ''b'')) \<rightarrow> (Add (var ''b'') (var ''a''))
+      where ((var ''a'')!; not (Number 0?)))"
+
+definition ShiftConstRight2 :: "StrategyRule" where
+  "ShiftConstRight2 = 
+    ((Add (var ''a'') (var ''b'')) \<rightarrow> (Add (var ''b'') (var ''a''))
+      where (condition (IsNumber (var ''a''))))"
+
+definition EvalMinus :: "StrategyRule" where
+  "EvalMinus = 
+    ((UMinus (Variable ''a'')) \<rightarrow> ((Variable ''b''))
+      where (condition (IsNumber (Variable ''a'')); func (UnaryMinus (Variable ''a'')); (Variable ''b'')?))"
+
+definition EvalMinus1 :: "StrategyRule" where
+  "EvalMinus1 =
+    (UMinus (Variable ''a'')) \<rightarrow> Variable ''b''
+      where (condition (IsNumber (Variable ''a'')); (Variable ''b'') := (func (UnaryMinus (Variable ''a''))))"
+
+definition EvalAdd :: "StrategyRule" where
+  "EvalAdd =
+    ((Add (Variable ''a'') (Variable ''b'')) \<rightarrow> ((Variable ''c''))
+      where (
+        (condition (IsNumber (Variable ''a'')));
+        (condition (IsNumber (Variable ''a'')));
+        ((Variable ''c'') := (func (Plus (Variable ''a'') (Variable ''b''))))
+      ))"
+
+subsubsection "Rewrite Application"
+
+text "
+The combination of @{term RedundantAdd} and @{term RedundantSub}
+provides us a rule that will eliminate zero in either add or sub expressions.
+It is defined as @{term \<open>RedundantAdd <+ RedundantSub\<close>}.
+The expanded version of this rule is:
+
+@{value \<open>RedundantAdd <+ RedundantSub\<close>}"
+
+\<comment> \<open>Failing to apply the rule\<close>
+value "eval (RedundantAdd <+ RedundantSub) ((Add (Number 10) (Number 10)), fmempty)"
+text \<open>@{value "eval (RedundantAdd <+ RedundantSub) ((Add (Number 10) (Number 10)), fmempty)"}\<close>
+
+\<comment> \<open>Successful application\<close>
+value "eval (RedundantAdd <+ RedundantSub) ((Add (Number 10) (Number 0)), fmempty)"
+text \<open>@{value "eval (RedundantAdd <+ RedundantSub) ((Add (Number 10) (Number 0)), fmempty)"}\<close>
+
+\<comment> \<open>Successful application in the second rule\<close>
+value "eval (RedundantSub <+ RedundantAdd) ((Add (Number 10) (Number 0)), fmempty)"
+text \<open>@{value "eval (RedundantSub <+ RedundantAdd) ((Add (Number 10) (Number 0)), fmempty)"}\<close>
+
+value "ShiftConstRight"
+value "eval ShiftConstRight ((Add (Number 0) (Number 10)), fmempty)"
+value "eval ShiftConstRight ((Add (Number 10) (Add (Number 10) (Number 20))), fmempty)"
+value "eval ShiftConstRight ((Add (Number 10) (Number 120)), fmempty)"
+
+value "eval ShiftConstRight2 ((Add (Number 0) (Number 10)), fmempty)"
+value "eval ShiftConstRight2 ((Add (Number 10) (Add (Number 10) (Number 20))), fmempty)"
+value "eval ShiftConstRight2 ((Add (Number 10) (Number 120)), fmempty)"
+
+value "eval EvalMinus ((UMinus (Number 10)), fmempty)"
+value "eval EvalMinus ((UMinus (Add (Number 10) (Number 10))), fmempty)"
+text \<open>@{value "eval EvalMinus ((UMinus (Number 10)), fmempty)"}\<close>
+
+value "eval EvalAdd ((UMinus (Number 10)), fmempty)"
+value "eval EvalAdd ((Add (Number 10) (Number 10)), fmempty)"
+text \<open>@{value "eval EvalAdd ((Add (Number 10) (Number 10)), fmempty)"}\<close>
+
+subsubsection \<open>Example: Match Pattern\<close>
+
+
+definition "join = Arithmetic.join"
+definition "generate = Arithmetic.generate"
+definition "match_pattern = Arithmetic.match_pattern"
+definition "optimized_export = Arithmetic.optimized_export"
+
+export_code "optimized_export" checking SML
+
+value "match_pattern
+(Sub (Add (Variable ''x'') (Variable ''y'')) (Variable ''y''))
+''e'' ({|''e''|}, Map.empty)"
+text \<open>@{value "match_pattern
+(Sub (Add (Variable ''x'') (Variable ''y'')) (Variable ''y''))
+''e'' ({|''e''|}, Map.empty)"}\<close>
+
+value "match_pattern
+(Sub 
+    (Add 
+        (Sub (Variable ''x'') (Variable ''x''))
+        (Sub (Variable ''y'') (Variable ''x'')))
+    (Variable ''y''))
+''e'' ({|''e''|}, Map.empty)"
+text \<open>@{value "match_pattern
+(Sub 
+    (Add 
+        (Sub (Variable ''x'') (Variable ''x''))
+        (Sub (Variable ''y'') (Variable ''x'')))
+    (Variable ''y''))
+''e'' ({|''e''|}, Map.empty)"}\<close>
+
+definition Identity where
+  "Identity = generate 
+    (Add
+      (var ''x'')
+      (Number 0))
+    (Result (var ''x''))"
+
+value "Identity"
+text "@{value[display] \<open>Identity\<close>}"
+value "optimized_export Identity"
+text "@{value[display] \<open>optimized_export Identity\<close>}"
+
+text \<open>@{text "const x + const y \<longrightarrow> const (x + y)"}\<close>
+definition Evaluate where
+  "Evaluate = generate 
+    (Add
+      (var ''x'')
+      (var ''y''))
+    (Result (var ''x''))"
+(* doesn't support constant evaluation *)
+value "Evaluate"
+value "(optimized_export (Evaluate))"
+
+text \<open>@{text "const x + y \<longrightarrow> y + const x when NotConst y"}\<close>
+definition LeftConst where
+  "LeftConst = generate 
+    (Add
+      (var ''x'')
+      (var ''y''))
+    (Plus (var ''y'') (var ''x''))"
+value "LeftConst"
+
+value "(choice [LeftConst, Evaluate, Identity])"
+text "@{value[display] \<open>choice [LeftConst, Evaluate, Identity]\<close>}"
+value "(optimized_export (choice [LeftConst, Evaluate, Identity]))"
+text "@{value[display] \<open>(optimized_export (choice [LeftConst, Evaluate, Identity]))\<close>}"
+value "(optimized_export (optimized_export (choice [LeftConst, Evaluate, Identity])))"
+text "@{value[display] \<open>(optimized_export (optimized_export (choice [LeftConst, Evaluate, Identity])))\<close>}"
+
+
+
+fun class_of_term_Arithmetic :: "Arithmetic \<Rightarrow> string" where
+  "class_of_term_Arithmetic (Add x y) = ''AddNode''" |
+  "class_of_term_Arithmetic (Sub x y) = ''SubNode''" |
+  "class_of_term_Arithmetic (UMinus x) = ''UnaryMinusNode''" |
+  "class_of_term_Arithmetic (Number v) = ''ConstantNode''" |
+  "class_of_term_Arithmetic (Variable s) = ''VariableNode''"
+
+datatype JavaCheck =
+  CallMethod1 |
+  CallMethod2 |
+  MethodCall string string |
+  Construct string "JavaCheck list" |
+  VariableExpr string
+
+instantiation "JavaCheck" :: JavaExpression
+begin
+fun expToJava_JavaCheck where
+  "expToJava_JavaCheck CallMethod1 = ''I'm asserting you're a number''" |
+  "expToJava_JavaCheck CallMethod2 = ''I'm asserting you're a subnode''" |
+  "expToJava_JavaCheck (MethodCall ob m) = ob @ ''.'' @ m @ ''()''" |
+  "expToJava_JavaCheck (Construct class args) = ''new '' @ class @ ''('' @ param_list (map expToJava_JavaCheck args) @ '')''" |
+  "expToJava_JavaCheck (VariableExpr v) = v"
+instance ..
+end
+
+fun generate_condition_Arithmetic :: "ArithmeticCondition \<Rightarrow> JavaCheck" where
+  "generate_condition_Arithmetic (IsSub e) = CallMethod2" |
+  "generate_condition_Arithmetic (IsNumber e) = CallMethod1"
+
+fun generate_Arithmetic :: "Arithmetic \<Rightarrow> JavaCheck" where
+  "generate_Arithmetic (Add x y) = Construct ''AddNode'' (map generate_Arithmetic [x, y])" |
+  "generate_Arithmetic (Sub x y) = Construct ''SubNode'' (map generate_Arithmetic [x, y])" |
+  "generate_Arithmetic (UMinus x) = Construct ''UnaryMinusNode'' (map generate_Arithmetic [x])" |
+  "generate_Arithmetic (Number v) = Construct ''ConstantNode'' []" |
+  "generate_Arithmetic (Variable s) = VariableExpr s"
+
+fun generate_result_Arithmetic :: "Transformer \<Rightarrow> JavaCheck" where
+  "generate_result_Arithmetic (UnaryMinus e) = CallMethod1" |
+  "generate_result_Arithmetic (Plus e1 e2) = CallMethod2" |
+  "generate_result_Arithmetic (Result e) = generate_Arithmetic e"
+
+fun generate_access_Arithmetic :: "VarName \<Rightarrow> Arithmetic \<Rightarrow> JavaCheck list" where
+  "generate_access_Arithmetic v (Add x y) = 
+    [(MethodCall v ''getX''),
+     (MethodCall v ''getY'')]" |
+  "generate_access_Arithmetic v (Sub x y) = 
+    [(MethodCall v ''getX''),
+     (MethodCall v ''getY'')]" |
+  "generate_access_Arithmetic v (UMinus x) = [(MethodCall v ''getValue'')]" |
+  "generate_access_Arithmetic v (Number val) = []" |
+  "generate_access_Arithmetic v (Variable s) = []"
+
+setup \<open>Locale_Code.open_block\<close>
+interpretation Arithmetic: JavaTarget
+  size_Arithmetic
+  "eval_condition"
+  "ground_condition"
+  "is_ground_condition"
+  "eval_transformer"
+  "ground_transformer"
+  "is_ground_transformer"
+  subexprs_Arithmetic
+  chain_Arithmetic
+  rewrite_Arithmetic
+  match_Arithmetic
+  varof_Arithmetic
+  var_Arithmetic
+  
+  class_of_term_Arithmetic
+  generate_condition_Arithmetic
+  generate_result_Arithmetic
+  generate_access_Arithmetic
+  by standard
+setup \<open>Locale_Code.close_block\<close>
+
+definition "export_rules = Arithmetic.export_rules"
+value "export_rules"
+
+value "export_rules (optimized_export (choice [Identity, Evaluate]))"
+value "export_rules (optimized_export (Identity \<then> Evaluate))"
+
+value "statementToJava 0 (export_rules (optimized_export (choice [Identity, Evaluate])))"
+
+
+end
